Tealeaves/Backends/DB/DB.v
@@ -1246,7 +1246,7 @@ Section theory.
       specialize (Hprem _ _ _ H0).
   Abort.
 
-  Lemma subst_pw_example (k: nat) (σ1 σ2 : nat -> T nat) (t: T nat):
+  Lemma subst_pointwise (k: nat) (σ1 σ2 : nat -> T nat) (t: T nat):
     cl_at k t ->
     (forall i, i < k -> σ1 i = σ2 i) ->
     subst σ1 t = subst σ2 t.
