Tealeaves/Examples/JAR/TranslateDemo.v
@@ -1,0 +1,37 @@
+From Tealeaves.Examples Require Import Lambda.Confluence.
+From Tealeaves.Backends Require Import LN DB.
+From Tealeaves.Backends.Adapters Require Import LNtoDB DBtoLN Roundtrips.LNDB.
+
+Check toLN: key -> lam nat -> option (lam LN).
+Check toDB: key -> lam LN  -> option (lam nat).
+
+Definition x: atom := 0.
+Definition y: atom := 1.
+Definition z: atom := 2.
+Definition a: atom := 3.
+Definition b: atom := 4.
+
+Example term1: lam LN := app (tvar (Bd 0)) (tvar (Fr x)).
+Example term2: lam LN := abs (app (tvar (Bd 0)) (tvar (Fr x))).
+Example term3: lam LN := abs (app (tvar (Fr z)) (tvar (Fr x))).
+Example term4: lam LN := abs (app (abs (abs (app (tvar (Fr z)) (tvar (Fr x))))) (app (tvar (Fr y)) (tvar (Fr a)))).
+
+Import List.ListNotations.
+
+Example k: key := [b; z; a; y; x].
+
+Compute toDB k term1.
+Compute map (toLN k) (toDB k term1).
+
+Compute toDB k term2.
+Compute map (toLN k) (toDB k term2).
+
+Compute toDB k term3.
+Compute map (toLN k) (toDB k term3).
+
+Compute toDB k term4.
+Compute map (toLN k) (toDB k term4).
+
+Goal map (toLN k) (toDB k term4) = Some (Some term4).
+  reflexivity.
+Qed.
